tmp

Register.v
@@ -175,45 +175,265 @@ Section Properties.
 Import LibEnv.
 
 Definition RegStateWF st :=
-  ok st.(requests) /\ ok st.(responses).
-  (* forall pid v, binds pid v st.(requests) -> pid # st.(responses) /\
-  forall pid v, binds pid v st.(responses) -> pid # st.(requests) *)
-  (* . *)
+  ok st.(requests) /\ ok st.(responses) /\
+  (forall pid v, binds pid v st.(requests) -> pid # st.(responses)) /\
+  (forall pid v, binds pid v st.(responses) -> pid # st.(requests))
+  .
+
+(* Lemma reg_ok_inv: invariant_ind Register RegStateWF.
+Proof.
+  unfold invariant_ind. intuition.
+  - inversion H; subst.
+    unfold RegStateWF.
+    unfold new_register.
+    simpl. intuition.
+    constructor.
+    constructor.
+    apply notin_empty.
+    apply notin_empty.
+  - unfold RegStateWF. inversion H0; subst; clear H0; simpl.
+    -- unfold RegStateWF in H; simpl in H.
+      intuition.
+      --- apply ok_remove in H2; eauto.
+      --- econstructor; eauto.
+      --- eapply notin_union; eauto.
+        assert (pid0 <> pid).
+        intro. subst.
+        eapply binds_fresh_inv in H5. intuition.
+        apply notin_concat.
+        eapply ok_middle_inv in H2; eauto.
+        assert (binds pid0 v0 (inv' ++ (pid, RegCAS old new) :: inv'')).
+        unfold binds.
+        rewrite get_notin_eq. assumption.
+        assumption.
+        apply H1 in H8. intuition.
+        apply notin_neq; auto.
+      --- unfold binds in H5. simpl in H5.
+        destruct (pid0 =? pid)eqn:Heq.
+        + apply Nat.eqb_eq in Heq. subst.
+          apply notin_concat.
+          eapply ok_middle_inv in H2; eauto.
+        + apply H6 in H5.
+          apply notin_concat.
+          apply notin_concat in H5. intuition.
+          apply notin_dom_push in H7. intuition.
+    -- unfold RegStateWF in H; simpl in H.
+      intuition.
+      --- apply ok_remove in H2; eauto.
+      --- econstructor; eauto.
+      --- eapply notin_union; eauto.
+        assert (pid0 <> pid).
+        intro. subst.
+        eapply binds_fresh_inv in H5. intuition.
+        apply notin_concat.
+        eapply ok_middle_inv in H2; eauto.
+        assert (binds pid0 v0 (inv' ++ (pid, RegRead) :: inv'')).
+        unfold binds.
+        rewrite get_notin_eq. assumption.
+        assumption.
+        apply H1 in H8. intuition.
+        apply notin_neq; auto.
+      --- unfold binds in H5. simpl in H5.
+        destruct (pid0 =? pid)eqn:Heq.
+        + apply Nat.eqb_eq in Heq. subst.
+          apply notin_concat.
+          eapply ok_middle_inv in H2; eauto.
+        + apply H6 in H5.
+          apply notin_concat.
+          apply notin_concat in H5. intuition.
+          apply notin_dom_push in H7. intuition.
+  - unfold RegStateWF. inversion H0; subst; clear H0; simpl.
+    -- unfold RegStateWF in H; simpl in H.
+      intuition.
+      --- econstructor; eauto.
+      --- unfold binds in H6; simpl in H6.
+        destruct (pid0 =? pid)eqn:Heq.
+        + apply Nat.eqb_eq in Heq; subst.
+          assumption.
+        + eapply H5; eassumption.
+      --- eapply notin_union; eauto.
+        assert (pid0 <> pid).
+        intro. subst.
+        eapply binds_fresh_inv in H6. intuition. assumption.
+        apply H7 in H6. intuition.
+        apply notin_neq; intuition.
+    -- unfold RegStateWF in H; simpl in H.
+      intuition.
+      --- econstructor; eauto.
+      --- unfold binds in H6; simpl in H6.
+        destruct (pid0 =? pid)eqn:Heq.
+        + apply Nat.eqb_eq in Heq; subst.
+          assumption.
+        + eapply H5; eassumption.
+      --- eapply notin_union; eauto.
+        assert (pid0 <> pid).
+        intro. subst.
+        eapply binds_fresh_inv in H6. intuition. assumption.
+        apply H7 in H6. intuition.
+        apply notin_neq; intuition.
+  - unfold RegStateWF. inversion H0; subst; clear H0; simpl.
+  - unfold RegStateWF. inversion H0; subst; clear H0; simpl.
+  - unfold RegStateWF. inversion H0; subst; clear H0; simpl.
+    -- unfold RegStateWF in H; simpl in H.
+      intuition.
+      --- apply ok_remove in H3; eauto.
+      --- apply H1 in H4.
+        apply notin_concat.
+        apply notin_concat in H4. intuition.
+        apply notin_dom_push in H6. intuition.
+      --- destruct (Nat.eq_dec pid0 pid).
+        + subst. apply ok_middle_inv in H3.
+          apply notin_concat in H3.
+          apply binds_fresh_inv in H4. inversion H4.
+          assumption.
+        + eapply H5.
+          unfold binds. rewrite get_notin_eq; intuition.
+          unfold binds; eassumption.
+    -- unfold RegStateWF in H; simpl in H.
+      intuition.
+      --- apply ok_remove in H3; eauto.
+      --- apply H1 in H4.
+        apply notin_concat.
+        apply notin_concat in H4. intuition.
+        apply notin_dom_push in H6. intuition.
+      --- destruct (Nat.eq_dec pid0 pid).
+        + subst. apply ok_middle_inv in H3.
+          apply notin_concat in H3.
+          apply binds_fresh_inv in H4. inversion H4.
+          assumption.
+        + eapply H5.
+          unfold binds. rewrite get_notin_eq; intuition.
+          unfold binds; eassumption.
+Qed. *)
+
+Definition _RegStateWF st :=
+  ok st.(requests) /\ ok st.(responses)
+  .
 
 Lemma reg_initial_preserves_ok: forall st st' pid qb,
-  initial_state Register st pid qb st' ->
   RegStateWF st ->
+  initial_state Register st pid qb st' ->
   RegStateWF st'.
 Proof.
+  - intros. unfold RegStateWF. inversion H0; subst; clear H0; simpl.
+    -- unfold RegStateWF in H; simpl in H.
+      intuition.
+      --- econstructor; eauto.
+      --- unfold binds in H6; simpl in H6.
+        destruct (pid0 =? pid)eqn:Heq.
+        + apply Nat.eqb_eq in Heq; subst.
+          assumption.
+        + eapply H5; eassumption.
+      --- eapply notin_union; eauto.
+        assert (pid0 <> pid).
+        intro. subst.
+        eapply binds_fresh_inv in H6. intuition. assumption.
+        apply H7 in H6. intuition.
+        apply notin_neq; intuition.
+    -- unfold RegStateWF in H; simpl in H.
+      intuition.
+      --- econstructor; eauto.
+      --- unfold binds in H6; simpl in H6.
+        destruct (pid0 =? pid)eqn:Heq.
+        + apply Nat.eqb_eq in Heq; subst.
+          assumption.
+        + eapply H5; eassumption.
+      --- eapply notin_union; eauto.
+        assert (pid0 <> pid).
+        intro. subst.
+        eapply binds_fresh_inv in H6. intuition. assumption.
+        apply H7 in H6. intuition.
+        apply notin_neq; intuition.
+Qed.
+        
+Lemma _reg_initial_preserves_ok: forall st st' pid qb,
+  initial_state Register st pid qb st' ->
+  _RegStateWF st ->
+  _RegStateWF st'.
+Proof.
   inversion 1; intros; subst;
-  unfold RegStateWF; simpl; intuition;
+  unfold _RegStateWF; simpl; intuition;
   econstructor; eauto.
 Qed.
 
 Lemma reg_final_preserves_ok: forall st st' pid rb,
-  final_state Register st pid rb st' ->
   RegStateWF st ->
+  final_state Register st pid rb st' ->
   RegStateWF st'.
 Proof.
+  - intros. unfold RegStateWF. inversion H0; subst; clear H0; simpl.
+    -- unfold RegStateWF in H; simpl in H.
+      intuition.
+      --- apply ok_remove in H3; eauto.
+      --- apply H1 in H4.
+        apply notin_concat.
+        apply notin_concat in H4. intuition.
+        apply notin_dom_push in H6. intuition.
+      --- destruct (Nat.eq_dec pid0 pid).
+        + subst. apply ok_middle_inv in H3.
+          apply notin_concat in H3.
+          apply binds_fresh_inv in H4. inversion H4.
+          assumption.
+        + eapply H5.
+          unfold binds. rewrite get_notin_eq; intuition.
+          unfold binds; eassumption.
+    -- unfold RegStateWF in H; simpl in H.
+      intuition.
+      --- apply ok_remove in H3; eauto.
+      --- apply H1 in H4.
+        apply notin_concat.
+        apply notin_concat in H4. intuition.
+        apply notin_dom_push in H6. intuition.
+      --- destruct (Nat.eq_dec pid0 pid).
+        + subst. apply ok_middle_inv in H3.
+          apply notin_concat in H3.
+          apply binds_fresh_inv in H4. inversion H4.
+          assumption.
+        + eapply H5.
+          unfold binds. rewrite get_notin_eq; intuition.
+          unfold binds; eassumption.
+Qed.
+
+Lemma _reg_final_preserves_ok: forall st st' pid rb,
+  final_state Register st pid rb st' ->
+  _RegStateWF st ->
+  _RegStateWF st'.
+Proof.
   inversion 1; intros; subst;
-  unfold RegStateWF; simpl; intuition;
+  unfold _RegStateWF; simpl; intuition;
   apply ok_remove in H2; intuition.
 Qed.
 
 Lemma reg_at_external_preserves_ok: forall st st' pid qa,
-  at_external Register st pid qa st' ->
   RegStateWF st ->
+  at_external Register st pid qa st' ->
   RegStateWF st'.
 Proof.
+  - intros. unfold RegStateWF. inversion H0; subst; clear H0; simpl.
+Qed.
+
+Lemma _reg_at_external_preserves_ok: forall st st' pid qa,
+  at_external Register st pid qa st' ->
+  _RegStateWF st ->
+  _RegStateWF st'.
+Proof.
   inversion 1; intros; subst;
-  unfold RegStateWF; simpl; intuition;
+  unfold _RegStateWF; simpl; intuition;
   apply ok_remove in H2; intuition.
 Qed.
 
 Lemma reg_after_external_preserves_ok: forall st st' pid ra,
-  after_external Register st pid ra st' ->
   RegStateWF st ->
+  after_external Register st pid ra st' ->
   RegStateWF st'.
+Proof.
+  - intros. unfold RegStateWF. inversion H0; subst; clear H0; simpl.
+Qed.
+
+Lemma _reg_after_external_preserves_ok: forall st st' pid ra,
+  after_external Register st pid ra st' ->
+  _RegStateWF st ->
+  _RegStateWF st'.
 Proof.
   inversion 1; intros; subst;
   unfold RegStateWF; simpl; intuition;
@@ -221,59 +441,72 @@ Proof.
 Qed.
 
 Lemma reg_step_preserves_ok: forall st st' pid int,
-  step Register st pid int st' ->
   RegStateWF st ->
+  step Register st pid int st' ->
   RegStateWF st'.
+Proof.
+  - intros. unfold RegStateWF. inversion H0; subst; clear H0; simpl.
+    -- unfold RegStateWF in H; simpl in H.
+      intuition.
+      --- apply ok_remove in H2; eauto.
+      --- econstructor; eauto.
+      --- eapply notin_union; eauto.
+        assert (pid0 <> pid).
+        intro. subst.
+        eapply binds_fresh_inv in H5. intuition.
+        apply notin_concat.
+        eapply ok_middle_inv in H2; eauto.
+        assert (binds pid0 v0 (inv' ++ (pid, RegCAS old new) :: inv'')).
+        unfold binds.
+        rewrite get_notin_eq. assumption.
+        assumption.
+        apply H1 in H8. intuition.
+        apply notin_neq; auto.
+      --- unfold binds in H5. simpl in H5.
+        destruct (pid0 =? pid)eqn:Heq.
+        + apply Nat.eqb_eq in Heq. subst.
+          apply notin_concat.
+          eapply ok_middle_inv in H2; eauto.
+        + apply H6 in H5.
+          apply notin_concat.
+          apply notin_concat in H5. intuition.
+          apply notin_dom_push in H7. intuition.
+    -- unfold RegStateWF in H; simpl in H.
+      intuition.
+      --- apply ok_remove in H2; eauto.
+      --- econstructor; eauto.
+      --- eapply notin_union; eauto.
+        assert (pid0 <> pid).
+        intro. subst.
+        eapply binds_fresh_inv in H5. intuition.
+        apply notin_concat.
+        eapply ok_middle_inv in H2; eauto.
+        assert (binds pid0 v0 (inv' ++ (pid, RegRead) :: inv'')).
+        unfold binds.
+        rewrite get_notin_eq. assumption.
+        assumption.
+        apply H1 in H8. intuition.
+        apply notin_neq; auto.
+      --- unfold binds in H5. simpl in H5.
+        destruct (pid0 =? pid)eqn:Heq.
+        + apply Nat.eqb_eq in Heq. subst.
+          apply notin_concat.
+          eapply ok_middle_inv in H2; eauto.
+        + apply H6 in H5.
+          apply notin_concat.
+          apply notin_concat in H5. intuition.
+          apply notin_dom_push in H7. intuition.
+Qed.
+
+Lemma _reg_step_preserves_ok: forall st st' pid int,
+  step Register st pid int st' ->
+  _RegStateWF st ->
+  _RegStateWF st'.
 Proof.
   inversion 1; intros; subst; simpl;
-  unfold RegStateWF; simpl; intuition;
+  unfold _RegStateWF; simpl; intuition;
   apply ok_remove in H1; intuition;
   econstructor; eauto.
-Qed.
-
-Lemma astep_preserves_ok: forall st st',
-  automaton_step Register st st' ->
-  RegStateWF st ->
-  RegStateWF st'.
-Proof.
-  intros. unfold automaton_step in H.
-  destruct H as [pid Htmp]. intuition.
-  - destruct H as [a Ha].
-    eapply reg_initial_preserves_ok; eauto.
-  - destruct H1 as [a Ha].
-    eapply reg_final_preserves_ok; eauto.
-  - destruct H as [a Ha].
-    eapply reg_at_external_preserves_ok; eauto.
-  - destruct H1 as [a Ha].
-    eapply reg_after_external_preserves_ok; eauto.
-  - destruct H1 as [a Ha].
-    eapply reg_step_preserves_ok; eauto.
-Qed.
-
-Lemma valid_execution_preserves_ok: forall st st' acts in_acts,
-  valid_execution_fragment Register st st' acts in_acts ->
-  RegStateWF st ->
-  RegStateWF st'.
-Proof.
-  induction 1; simpl; intros.
-  - subst; auto.
-  - eapply reg_step_preserves_ok in H; eauto.
-  - eapply reg_at_external_preserves_ok in H; eauto.
-  - eapply reg_after_external_preserves_ok in H; eauto.
-  - eapply reg_initial_preserves_ok in H; eauto.
-  - eapply reg_final_preserves_ok in H; eauto.
-Qed.
-  
-Lemma reachable_inv: forall st,
-  reachable Register st ->
-  RegStateWF st.
-Proof.
-  intros. unfold reachable in H.
-  destruct H as [init [acts [in_acts [Hnew Hexe]]]].
-  eapply valid_execution_preserves_ok; eauto.
-  inversion Hnew; subst.
-  unfold new_register.
-  unfold RegStateWF. simpl. intuition; econstructor.
 Qed.
 
 Lemma reg_ok_inv: invariant_ind Register RegStateWF.
@@ -282,12 +515,75 @@ Proof.
   - inversion H; subst.
     unfold RegStateWF.
     unfold new_register.
-    simpl. constructor; constructor.
+    simpl. intuition.
+    constructor.
+    constructor.
+    apply notin_empty.
+    apply notin_empty.
   - eapply reg_step_preserves_ok; eauto.
   - eapply reg_initial_preserves_ok; eauto.
   - eapply reg_at_external_preserves_ok; eauto.
   - eapply reg_after_external_preserves_ok; eauto.
   - eapply reg_final_preserves_ok; eauto.
+Qed.
+
+Lemma astep_preserves_ok: forall st st',
+  automaton_step Register st st' ->
+  _RegStateWF st ->
+  _RegStateWF st'.
+Proof.
+  intros. unfold automaton_step in H.
+  destruct H as [pid Htmp]. intuition.
+  - destruct H as [a Ha].
+    eapply _reg_initial_preserves_ok; eauto.
+  - destruct H1 as [a Ha].
+    eapply _reg_final_preserves_ok; eauto.
+  - destruct H as [a Ha].
+    eapply _reg_at_external_preserves_ok; eauto.
+  - destruct H1 as [a Ha].
+    eapply _reg_after_external_preserves_ok; eauto.
+  - destruct H1 as [a Ha].
+    eapply _reg_step_preserves_ok; eauto.
+Qed.
+
+Lemma valid_execution_preserves_ok: forall st st' acts in_acts,
+  valid_execution_fragment Register st st' acts in_acts ->
+  _RegStateWF st ->
+  _RegStateWF st'.
+Proof.
+  induction 1; simpl; intros.
+  - subst; auto.
+  - eapply _reg_step_preserves_ok in H; eauto.
+  - eapply _reg_at_external_preserves_ok in H; eauto.
+  - eapply _reg_after_external_preserves_ok in H; eauto.
+  - eapply _reg_initial_preserves_ok in H; eauto.
+  - eapply _reg_final_preserves_ok in H; eauto.
+Qed.
+  
+Lemma reachable_inv: forall st,
+  reachable Register st ->
+  _RegStateWF st.
+Proof.
+  intros. unfold reachable in H.
+  destruct H as [init [acts [in_acts [Hnew Hexe]]]].
+  eapply valid_execution_preserves_ok; eauto.
+  inversion Hnew; subst.
+  unfold new_register.
+  unfold _RegStateWF. simpl. intuition; econstructor.
+Qed.
+
+Lemma _reg_ok_inv: invariant_ind Register _RegStateWF.
+Proof.
+  unfold invariant_ind. intuition.
+  - inversion H; subst.
+    unfold RegStateWF.
+    unfold new_register.
+    simpl. constructor; constructor.
+  - eapply _reg_step_preserves_ok; eauto.
+  - eapply _reg_initial_preserves_ok; eauto.
+  - eapply _reg_at_external_preserves_ok; eauto.
+  - eapply _reg_after_external_preserves_ok; eauto.
+  - eapply _reg_final_preserves_ok; eauto.
 Qed.
 
 Lemma binds_same: forall (req: env Register_query) pid qb qb',
@@ -381,14 +677,14 @@ Qed.
 Lemma internal_preserves_request: forall acts in_acts pid st st' qb qb',
   gather_pid_external_events acts pid = [] ->
   binds pid qb st.(requests) ->
-  RegStateWF st ->
+  _RegStateWF st ->
   binds pid qb' st'.(requests) ->
   valid_execution_fragment Register st st' acts in_acts ->
   qb = qb'.
 Proof.
   intros. induction H3.
   - subst. eapply binds_same; eauto.
-    unfold RegStateWF in H1; intuition.
+    unfold _RegStateWF in H1; intuition.
   - eapply IHvalid_execution_fragment; eauto.
     destruct (pid =? pid0)eqn:Heq.
     -- assert (pid # st'.(requests)).
@@ -410,7 +706,7 @@ Proof.
       + simpl in H0.
         eapply binds_remove with (E2:=[(pid0, RegRead)]); simpl; eauto.
         apply notin_neq. apply Nat.eqb_neq. assumption.
-    -- eapply reg_step_preserves_ok; eauto.
+    -- eapply _reg_step_preserves_ok; eauto.
   - inversion H3.
   - inversion H3.
   - simpl in H.
@@ -419,14 +715,14 @@ Proof.
     -- apply IHvalid_execution_fragment; auto.
       eapply initial_preserves_binds; eauto.
       apply Nat.eqb_neq; auto.
-      eapply reg_initial_preserves_ok; eauto.
+      eapply _reg_initial_preserves_ok; eauto.
   - simpl in H.
     destruct (pid =? pid0)eqn:Heq.
     -- inversion H.
     -- apply IHvalid_execution_fragment; auto.
       eapply final_preserves_binds; eauto.
       apply Nat.eqb_neq; auto.
-      eapply reg_final_preserves_ok; eauto.
+      eapply _reg_final_preserves_ok; eauto.
 Qed.
 
 End Properties.
